glue code between the plugin and Ltac2

plugin/evaluation.ml
@@ -18,14 +18,14 @@ struct
   (**************************************************************************************)
 
   (** Pattern which matches [O.E_Var ?i]. *)
-  let e_var_patt : EConstr.t patt =
+  let var_patt : EConstr.t patt =
    fun t env sigma ->
     match EConstr.kind sigma t with
     | App (f, [| i |]) when is_ctor sigma P.ops1.e_var f -> (sigma, Some i)
     | _ -> (sigma, None)
 
   (** Pattern which matches [O.E_ctor ?c ?al]. *)
-  let e_ctor_patt : (EConstr.t * EConstr.t) patt =
+  let ctor_patt : (EConstr.t * EConstr.t) patt =
    fun t env sigma ->
     match EConstr.kind sigma t with
     | App (f, [| c; al |]) when is_ctor sigma P.ops1.e_ctor f -> (sigma, Some (c, al))
@@ -73,15 +73,15 @@ struct
   (** *** Reify terms and substitutions. *)
   (**************************************************************************************)
 
-  let rec eval_term (t : EConstr.t) : (EConstr.t * EConstr.t) m =
-    (* Branch for [Var ?i]. *)
+  let rec eval_term (t' : EConstr.t) : (EConstr.t * EConstr.t) m =
+    (* Branch for [O.E_Var ?i]. *)
     let var_branch i =
-      let t' = app (mkctor P.ops1.e_var) i in
+      let t = app (mkctor (P.ops0.term, 1)) i in
       let* p = apps_ev (Lazy.force Consts.eq_refl) 1 [| t |] in
-      ret (t', p)
+      ret (t, p)
     in
     (* Branch for [C_i ?args]. *)
-    let ctor_branch (i, args) : (EConstr.t * EConstr.t) m =
+    (*let ctor_branch (i, args) : (EConstr.t * EConstr.t) m =
       let args = Array.to_list args in
       (* Reify a single argument. *)
       let rec reify_arg (ty, arg) =
@@ -116,19 +116,19 @@ struct
         apps_ev (mkconst P.congr.congr_ctors.(i)) (2 * n_args) @@ Array.of_list p_args
       in
       ret (t', p)
-    in
-    (* Branch for [rename ?r ?t1]. *)
-    let rename_branch (r, t1) =
+    in*)
+    (* Branch for [O.rename ?r ?t1']. *)
+    let rename_branch (r, t1') =
       let* p_r = apps_ev (Lazy.force Consts.reflexivity) 3 [| r |] in
-      let* t1', p_t1 = reify_term t1 in
-      let t' = apps (mkconst P.ops1.rename) [| kt P.ops1; r; t1' |] in
+      let* t1, p_t1 = eval_term t1' in
+      let t = apps (mkconst P.ops0.rename) [| r; t1 |] in
       let p1 = apps (mkconst P.pe.eval_rename) [| r; t1' |] in
       let* p2 = apps_ev (mkconst P.congr.congr_rename) 4 [| p_r; p_t1 |] in
       let* p = apps_ev (Lazy.force Consts.transitivity) 6 [| p1; p2 |] in
-      ret (t', p)
+      ret (t, p)
     in
     (* Branch for [substitute ?s ?t1]. *)
-    let substitute_branch (s, t1) =
+    (*let substitute_branch (s, t1) =
       let* s', p_s = reify_subst s in
       let* t1', p_t1 = reify_term t1 in
       let t' = apps (mkconst P.ops1.substitute) [| kt P.ops1; s'; t1' |] in
@@ -136,23 +136,19 @@ struct
       let* p2 = apps_ev (mkconst P.congr.congr_substitute) 4 [| p_s; p_t1 |] in
       let* p = apps_ev (Lazy.force Consts.transitivity) 6 [| p1; p2 |] in
       ret (t', p)
-    in
+    in*)
     (* Default branch. *)
-    let default_branch t =
-      let t' = app (mkconst P.re.reify) t in
+    let default_branch t' =
+      let t = apps (mkconst P.re.eval) [| kt P.ops1; t' |] in
       let p = app (mkconst P.bij.eval_reify_inv) t in
-      ret (t', p)
+      ret (t, p)
     in
     (* Actual pattern matching. *)
-    pattern_match t
-      [ Case (var_patt, var_branch)
-      ; Case (ctor_patt, ctor_branch)
-      ; Case (rename_patt, rename_branch)
-      ; Case (substitute_patt, substitute_branch)
-      ]
+    pattern_match t'
+      [ Case (var_patt, var_branch); Case (rename_patt, rename_branch) ]
       default_branch
 
-  and reify_subst (s : EConstr.t) : (EConstr.t * EConstr.t) m =
+  (*and eval_subst (s : EConstr.t) : (EConstr.t * EConstr.t) m =
     (* Match [sid]. *)
     let sid_branch () =
       let s' = mkconst P.ops1.sid in
@@ -198,5 +194,39 @@ struct
       ; Case (scons_patt, scons_branch)
       ; Case (scomp_patt, scomp_branch)
       ]
-      default_branch
+      default_branch*)
 end
+
+(**************************************************************************************)
+(** *** Putting it all together. *)
+(**************************************************************************************)
+
+(** [eval_term sign ops t'] evaluates the level zero one [t'] into a pair [(t, p)]:
+    - [t] is a level zero term.
+    - [p] is a proof of [eval t' = t]. *)
+let eval_term (sign : signature) (ops : ops_all) (t' : EConstr.t) :
+    (EConstr.t * EConstr.t) m =
+  let* env = get_env in
+  let* sigma = get_sigma in
+  Log.printf "%s" (Log.show_econstr env sigma t');
+  let module M = Make (struct
+    let sign = sign
+    let ops0 = ops.ops_ops0
+    let ops1 = ops.ops_ops1
+    let congr = ops.ops_congr
+    let re = ops.ops_re
+    let bij = ops.ops_bij
+    let pe = ops.ops_pe
+  end) in
+  let* t, p = M.eval_term t' in
+  (* Typecheck to resolve evars. *)
+  let* _ = typecheck t None in
+  let p_ty =
+    apps (Lazy.force Consts.eq)
+      [| mkind ops.ops_ops0.term
+       ; apps (mkconst ops.ops_re.eval) [| kt ops.ops_ops1; t' |]
+       ; t
+      |]
+  in
+  let* _ = typecheck p (Some p_ty) in
+  ret (t, p)
