plugin/main.ml
@@ -1,4 +1,5 @@
 open Prelude
+open Ltac2_plugin
 
 (** A testing signature.*)
 let build_signature () : signature =
@@ -89,7 +90,7 @@ let generate_operations (s : signature) : ops_all =
   }
 
 (** Main entry point for the plugin. *)
-let main () =
+let generate () =
   (* We use a testing signature (for the moment). *)
   let s = build_signature () in
   (* Generate the operations. *)
@@ -114,5 +115,49 @@ let reify (t : Constrexpr.constr_expr) : unit =
   let* env = get_env in
   let* sigma = get_sigma in
   Log.printf "reify result: %s" (Log.show_econstr env sigma t');
+  Log.printf "type of the proof: %s" (Log.show_econstr env sigma p_ty);
+  ret ()
+
+let reify_tac (t0 : EConstr.t) : (EConstr.t * EConstr.t) Proofview.tactic =
+  let open PVMonad in
+  let s = build_signature () in
+  let ops =
+    match !saved_ops with
+    | None -> Log.error "reify_tac: must generate operations beforehand."
+    | Some ops -> ops
+  in
+  Proofview.Goal.enter_one @@ fun g ->
+  (* Level 0 -> Level 1 *)
+  let env = Proofview.Goal.env g in
+  let sigma = Proofview.Goal.sigma g in
+  let sigma, res = Reification.reify_term s ops t0 env sigma in
+  let* _ = Proofview.Unsafe.tclEVARSADVANCE sigma in
+  ret res
+
+let tac_name (s : string) : Tac2expr.ml_tactic_name =
+  { mltac_plugin = "autosubst-experiments.plugin"; mltac_tactic = s }
+
+let () =
+  let open Tac2externals in
+  let open Tac2ffi in
+  define (tac_name "reify") (constr @-> tac (pair constr constr)) @@ fun t0 ->
+  reify_tac t0
+
+let eval (t' : Constrexpr.constr_expr) : unit =
+  let s = build_signature () in
+  let ops =
+    match !saved_ops with
+    | None -> Log.error "reify: must generate operations beforehand."
+    | Some ops -> ops
+  in
+  monad_run
+  @@
+  (* Reify. *)
+  let* t' = pretype t' in
+  let* t, p = Evaluation.eval_term s ops t' in
+  let* p_ty = retype p in
+  (* Print. *)
+  let* env = get_env in
+  let* sigma = get_sigma in
   Log.printf "type of the proof: %s" (Log.show_econstr env sigma p_ty);
   ret ()
