theories/Test.v
@@ -1,61 +1,78 @@
-From Coq Require Import Lia.
-From Coq Require Import String.
+From Coq Require Import Lia String.
+From Ltac2 Require Ltac2.
+From Ltac2 Require Import Printf.
 From Prototype Require Import Prelude Sig.
 From Prototype Require Constants LevelOne LevelTwo LevelTwoIrred LevelTwoSimp.
 
 Declare ML Module "autosubst-experiments.plugin".
+Ltac2 @external reify : constr -> constr * constr := "autosubst-experiments.plugin" "reify".
 
-Test.
+Autosubst Generate.
 
-(*Reify (substitute (scomp sid (scons (Var 0) sid)) (Var 0)).*)
-(*Reify (rename (rcomp rid rshift) (Var 0)).*)
-Reify (Lam "x" (Var 0)).
+Class TermSimplification (t s : term) := 
+  MkTermSimplification { term_simplification : t = s }.
 
-(*Print term.
-Print rename.
-Print subst.
-Print srcomp.
-Print rscomp.
-Print sid.
-Print sshift.
-Print scons.
-Print up_subst.
-Print substitute.
-Print scomp.*)
+Arguments term_simplification t {s _}.
+Hint Mode TermSimplification + - : typeclass_instances.
 
-(*About congr_App.
-About congr_Lam.
-About congr_rename.
-About congr_rscomp.
-About congr_srcomp.
-About congr_scons.
-About congr_up_subst.
-About congr_substitute.
-About congr_scomp.*)
+Lemma autosubst_simpl_term_substitute s t res :
+  TermSimplification (substitute s t) res -> substitute s t = res.
+Proof. intros H. now apply term_simplification. Qed.
+#[export] Hint Rewrite -> autosubst_simpl_term_substitute : asimpl.
 
-(*Print base.
-Print eval_base.
-Print ctor.
-Print ctor_type.
-Print S.t.
-About T.*)
+Lemma congr_eval : 
+  forall k (t1 t2 : T.O.expr k), t1 = t2 -> eval k t1 = eval k t2.
+Proof. now intros k t1 t2 ->. Qed.
 
-(*Print reify.
-Print sreify.
-Print eval_arg.
-Print eval_args.
-Print eval_kind.
-Print eval_ctor.
-Print eval.*)
+From Ltac2 Require Import RedFlags.
 
-(*About eval_reify_inv.
-About seval_sreify_inv.
-About term_ind'.*)
+Ltac2 rasimpl_red_flags () : RedFlags.t := 
+  red_flags:(beta delta [T.eeval]).
 
-(*About eval_rename.
-About seval_rscomp.
-About seval_srcomp.
-About seval_scons.
-About seval_up_subst.
-About eval_substitute.
-About seval_scomp.*)
+
+(** Solve a goal of the form [TermSimplification t0]. *)
+Ltac2 build_TermSimplification (t0 : constr) : unit :=
+  (* Reify Level 0 -> Level 1. *)
+  let (t1, p1) := reify t0 in 
+  let p1 := constr:(eq_sym $p1) in
+  printf "t1 := %t" t1;
+  printf "p1 := %t" (Constr.type p1);
+  (* Reify Level 1 -> Level 2. *)
+  let env := T.empty_env () in
+  let (env, t2) := T.reify_expr env t1 in
+  let env := T.build_env env in
+  printf "t2 := %t" t2;
+  (* Simplify. *)
+  let t2' := constr:(T.esimp $t2) in
+  let p2 := constr:(eq_sym (T.esimp_sound $env $t2)) in
+  printf "t2' := %t" t2';
+  printf "p2 := %t" p2;
+  let t2'' := Std.eval_cbn rasimpl_red_flags t2 in 
+  (* Build the instance of [TermSimplification t0]. *)
+  let t0' := constr:(eval Kt (T.eeval $env $t2')) in
+  let eq := constr:(eq_trans $p1 (congr_eval Kt $t1 _ $p2)) in
+  printf "t0' := %t" t0';
+  exact (MkTermSimplification $t0 $t0' $eq).
+  
+#[export] Hint Extern 10 (TermSimplification ?t0 _) =>
+  let tac := ltac2:(t0 |-  
+    match Ltac1.to_constr t0 with 
+    | Some t0 => build_TermSimplification t0
+    | None => Control.throw_invalid_argument "build_TermSimplification"
+    end) 
+  in 
+  tac t0 : typeclass_instances.
+    
+Ltac rasimpl := (rewrite_strat (topdown (hints asimpl))) ; [ | (exact _) ..].
+
+Lemma test : substitute sid (substitute (scomp sshift sid) (Var 0)) = Var 0.
+Proof. rasimpl.
+
+Qed.
+
+
+
+(*Autosubst Reify (substitute (scomp sid (scons (Var 0) sid)) (Var 0)).*)
+(*Autosubst Reify (rename (rcomp rid rshift) (Var 0)).*)
+(*Autosubst Reify (Lam "x" (Var 0)).*)
+(*Autosubst Eval (T.O.E_var 0).*)
